theories/iSL/Order.v
@@ -1,82 +1,118 @@
-Require Export ISL.Environments.
+Require Export ISL.SizedFormulas ISL.Formulas.
+Require Export List.
+Require Export stdpp.gmultiset.
+Require Import Coq.Program.Equality.
+
+Section Definitions.
+
+Set Implicit Arguments.
+Variable p : variable.
+
+
+Definition form_of_sig (s : {n & @nform p n}) : form := let (x, n) := s in form_of_nform n.
+Definition senv  := list {n & @nform p n}.
+
+Definition pow_weight nφ := 5^ weight (form_of_sig nφ).
 
 (* Note 3 or 4 would suffice for IPC ; iSL requires 5 *)
-Definition env_weight (Γ : env) := list_sum (map (fun x => 5^ weight x) (elements Γ)).
+Definition senv_weight (Γ : senv) := list_sum (map pow_weight Γ).
 
-Lemma env_weight_disj_union Γ Δ : env_weight (disj_union Γ Δ) = env_weight Γ +  env_weight Δ.
+Lemma senv_weight_disj_union Γ Δ : senv_weight (Γ ++  Δ) = senv_weight Γ +  senv_weight Δ.
 Proof. 
-unfold env_weight. 
-assert (Heq := gmultiset_elements_disj_union Γ Δ).
-apply (Permutation_map (λ x : form, 5 ^ weight x)) in Heq.
-apply Permutation_list_sum in Heq.
-rewrite map_app, list_sum_app in Heq. exact Heq.
+unfold senv_weight. 
+now rewrite map_app, list_sum_app.
 Qed.
 
-Lemma env_weight_add Γ φ : env_weight (Γ • φ) = env_weight Γ +  (5 ^ weight φ).
+Lemma senv_weight_add (Γ : senv) φ : senv_weight ((φ :: Γ)) = pow_weight φ + senv_weight Γ.
 Proof.
-rewrite env_weight_disj_union. unfold env_weight at 2.
-setoid_rewrite gmultiset_elements_singleton. simpl. lia.
+unfold senv_weight. simpl. lia.
 Qed.
 
-Global Hint Rewrite env_weight_add : order.
-
-Definition env_order := ltof env env_weight.
-Infix "≺" := env_order (at level 150).
-
-Lemma env_weight_singleton (φ : form) : env_weight {[ φ ]} = 5 ^ weight φ.
+Lemma senv_weight_remove_le Δ φ:
+  senv_weight (remove (nform_eq_dec p) φ Δ) ≤ senv_weight Δ.
 Proof.
-unfold env_weight, ltof.
-replace (elements {[ φ ]}) with [φ]. simpl. lia. now rewrite <- gmultiset_elements_singleton.
+induction Δ as [|φ' Δ HΔ]; trivial.
+simpl. case nform_eq_dec;
+intro; subst; repeat rewrite senv_weight_add; lia.
 Qed.
 
-Lemma env_order_singleton (φ ψ : form) : weight φ < weight ψ -> {[+ φ +]}≺ {[+ ψ +]}.
+
+Lemma senv_weight_open_boxes Δ : senv_weight (□⁻¹ Δ) ≤ senv_weight Δ. 
 Proof.
-intro Hw. unfold env_order, ltof. do 2 rewrite env_weight_singleton.
+unfold senv_weight.
+induction Δ as [|[n φ] Δ]; simpl. lia.
+apply Nat.add_le_mono; trivial.
+apply Nat.pow_le_mono_r. lia.
+simpl. destruct φ; simpl; constructor; trivial.
+Qed.
+
+Lemma pow_weight_gt φ : 5 <= 5 ^ weight φ.
+Proof.
+  rewrite <- (Nat.pow_1_r 5) at 1.
+  apply Nat.pow_le_mono_r. lia. apply weight_pos.
+Qed.
+
+Definition senv_order := ltof senv senv_weight.
+Infix "≺" := senv_order (at level 150).
+
+Lemma senv_weight_singleton φ : senv_weight [ φ ] = 5 ^ weight (form_of_sig φ).
+Proof.
+unfold senv_weight, ltof. simpl. unfold pow_weight; lia.
+Qed.
+(*
+Lemma env_order_singleton (φ ψ : form) : weight φ < weight ψ -> [ φ +]}≺ {[+ ψ +]}.
+Proof.
+intro Hw. unfold env_order, ltof. do 2 rewrite senv_weight_singleton.
 apply Nat.pow_lt_mono_r. lia. trivial.
 Qed.
-
+*)
 Notation "Δ ≼ Δ'" := ((Δ ≺ Δ') \/ Δ = Δ') (at level 150).
 
-Lemma env_le_weight Δ Δ' : (Δ' ≼ Δ) -> env_weight Δ' ≤ env_weight Δ.
+Lemma senv_le_weight Δ Δ' : (Δ' ≼ Δ) -> senv_weight Δ' ≤ senv_weight Δ.
 Proof.
-unfold env_order. intros [Hle | Heq].
+unfold senv_order. intros [Hle | Heq].
 - auto with *.
 - subst; trivial.
 Qed.
 
-Global Hint Resolve env_le_weight : order.
+Global Instance senv_order_trans : Transitive senv_order.
+Proof. unfold senv_order, senv_weight, ltof. auto with *. Qed.
 
-Global Hint Unfold form_order : mset.
-
-
-Global Instance env_order_trans : Transitive env_order.
-Proof. unfold env_order, env_weight, ltof. auto with *. Qed.
-
-Definition wf_env_order : well_founded env_order.
-Proof. now apply well_founded_lt_compat with env_weight.
+Definition wf_senv_order : well_founded senv_order.
+Proof. now apply well_founded_lt_compat with senv_weight.
 Defined.
 
 (* We introduce a notion of "pointed" environment, which is simply
  * a pair (Δ, φ), where Δ is an environment and φ is a formula,
  * not necessarily an element of Δ.  *)
-Definition pointed_env := (env * form)%type.
+Definition pointed_senv := (senv * {n & @nform p n})%type.
 
 (* The order on pointed environments is given by considering the
  * environment order on the sum of Δ and {φ}. *)
  (* TODO: modified from G4IP : right-hand side counts twice, to account for the right box rule. Is this working? *)
-Definition pointed_env_order (pe1 : pointed_env) (pe2 : pointed_env) :=
-  env_order (fst pe1 • snd pe1 • snd pe1) (fst pe2 • snd pe2 •  snd pe2).
+Definition pointed_senv_order (pe1 : pointed_senv) (pe2 : pointed_senv) :=
+  senv_order (snd pe1 :: snd pe1 :: fst pe1) (snd pe2 :: snd pe2 :: fst pe2).
 
-Lemma wf_pointed_order : well_founded pointed_env_order.
+Lemma wf_pointed_order : well_founded pointed_senv_order.
 Proof. apply well_founded_ltof. Qed.
 
-Infix "≺·" := pointed_env_order (at level 150).
+(*
+Global Instance Proper_senv_order : Proper ((≡@{senv}) ==> (≡@{senv}) ==> (fun x y => x <-> y)) senv_order.
+Proof. intros Δ1 Δ2 H12 Δ3 Δ4 H34.
+unfold senv_order, ltof,senv_weight.
+unfold equiv, sets.set_equiv_instance in *.
+ apply Permutation_list_sum in H12.
+ Qed.
 
-Lemma env_order_equiv_right_compat {Δ Δ' Δ'' : env}:
+Lemma env_order_equiv_right_compat {Δ Δ' Δ'' : senv}:
   Δ' ≡ Δ'' ->
   (Δ ≺ Δ'') ->
   Δ ≺ Δ'.
-Proof. ms. Qed.
+Proof. unfold senv_order, ltof. unfold equiv.
+
+ multiset_solver. Qed.
+
+
 
 Lemma env_order_equiv_left_compat {Δ Δ' Δ'' : env}:
   Δ ≡ Δ'' ->
@@ -84,13 +120,11 @@ Lemma env_order_equiv_left_compat {Δ Δ' Δ'' : env}:
   Δ ≺ Δ'.
 Proof. ms. Qed.
 
-Global Instance Proper_env_order : Proper ((≡@{env}) ==> (≡@{env}) ==> (fun x y => x <-> y)) env_order.
-Proof. intros Δ1 Δ2 H12 Δ3 Δ4 H34; ms. Qed.
-
-
+*)
+(*
 Lemma env_order_1  Δ φ1 φ : weight φ1 < weight φ -> Δ • φ1 ≺ Δ • φ.
 Proof.
-intros Hw.  unfold env_order, ltof. do 2 rewrite env_weight_add.
+intros Hw.  unfold env_order, ltof. do 2 rewrite senv_weight_add.
 apply Nat.add_lt_mono_l. apply Nat.pow_lt_mono_r. lia. trivial.
 Qed.
 
@@ -98,23 +132,24 @@ Local Hint Resolve Nat.pow_lt_mono_r : order.
 
 Lemma env_order_compat  Δ Δ' φ1 φ : weight φ1 < weight φ -> (Δ' ≼ Δ) -> Δ' • φ1 ≺ Δ • φ.
 Proof.
-intros.  unfold env_order, ltof. repeat rewrite env_weight_add.
+intros.  unfold env_order, ltof. repeat rewrite senv_weight_add.
 apply Nat.add_le_lt_mono; auto with *.
 Qed.
 
 Global Hint Resolve env_order_compat : order.
-
-Lemma env_order_add_compat Δ Δ' φ : (Δ ≺ Δ') -> (Δ • φ) ≺ (Δ' • φ).
+*)
+Lemma env_order_add_compat Δ Δ' φ : (Δ ≺ Δ') -> (φ :: Δ) ≺ (φ :: Δ').
 Proof.
-unfold env_order, ltof. do 2 rewrite env_weight_add. lia.
+unfold senv_order, ltof. do 2 rewrite senv_weight_add. lia.
 Qed.
-
+(*
 (* TODO: this is just a special case *)
 Lemma env_order_disj_union_compat_left Δ Δ' Δ'':
   (Δ ≺ Δ'') -> Δ ⊎ Δ' ≺ Δ'' ⊎ Δ'.
 Proof.
-unfold env_order, ltof. intro. do 2 rewrite env_weight_disj_union. lia.
+unfold env_order, ltof. intro. do 2 rewrite senv_weight_disj_union. lia.
 Qed.
+
 
 Lemma env_order_disj_union_compat_right Δ Δ' Δ'':
   (Δ ≺ Δ'') -> Δ' ⊎ Δ ≺ Δ' ⊎ Δ''.
@@ -139,7 +174,7 @@ Lemma env_order_disj_union_compat_strong_right Δ Δ' Δ'' Δ''':
 Proof.
 intros H1 H2. 
 destruct H2 as [Hlt|Heq].
-- unfold env_order, ltof in *. do 2 rewrite env_weight_disj_union. lia.
+- unfold env_order, ltof in *. do 2 rewrite senv_weight_disj_union. lia.
 - rewrite Heq. now apply env_order_disj_union_compat_left.
 Qed.
 
@@ -148,7 +183,7 @@ Lemma env_order_disj_union_compat_strong_left Δ Δ' Δ'' Δ''':
 Proof.
 intros H1 H2. 
 destruct H1 as [Hlt|Heq].
-- unfold env_order, ltof in *. do 2 rewrite env_weight_disj_union. lia.
+- unfold env_order, ltof in *. do 2 rewrite senv_weight_disj_union. lia.
 - rewrite Heq. now apply env_order_disj_union_compat_right.
 Qed.
 
@@ -173,7 +208,7 @@ Global Hint Resolve open_boxes_env_order : order.
 
 Lemma env_order_0 Δ φ: Δ ≺ Δ • φ.
 Proof.
-unfold env_order, ltof. rewrite env_weight_disj_union, env_weight_singleton.
+unfold env_order, ltof. rewrite senv_weight_disj_union, senv_weight_singleton.
 apply Nat.lt_add_pos_r. transitivity (5 ^ 0). simpl. lia. apply Nat.pow_lt_mono_r. lia.
 apply weight_pos.
 Qed.
@@ -192,8 +227,8 @@ Lemma env_order_2  Δ Δ' φ1 φ2 φ: weight φ1 < weight φ -> weight φ2 < wei
   (Δ' ≼ Δ) -> Δ' • φ1 • φ2 ≺ Δ • φ.
 Proof.
 intros Hw1 Hw2 Hor.
-unfold env_order, ltof. repeat rewrite env_weight_add.
-apply env_le_weight in Hor.
+unfold env_order, ltof. repeat rewrite senv_weight_add.
+apply senv_le_weight in Hor.
 replace (weight φ) with (S (pred (weight φ))) by lia.
 apply Nat.lt_le_pred in Hw1, Hw2.
 simpl. repeat rewrite Nat.add_assoc.
@@ -209,8 +244,8 @@ Lemma env_order_3  Δ Δ' φ1 φ2 φ3 φ:
   Δ' • φ1 • φ2  • φ3 ≺ Δ • φ.
 Proof.
 intros Hw1 Hw2 Hw3 Hor.
-unfold env_order, ltof. repeat rewrite env_weight_add.
-apply env_le_weight in Hor.
+unfold env_order, ltof. repeat rewrite senv_weight_add.
+apply senv_le_weight in Hor.
 replace (weight φ) with (S (pred (weight φ))) by lia.
 apply Nat.lt_le_pred in Hw1, Hw2.
 simpl. repeat rewrite Nat.add_assoc.
@@ -226,8 +261,8 @@ Lemma env_order_4  Δ Δ' φ1 φ2 φ3 φ4 φ:
    (Δ' ≼ Δ) -> Δ' • φ1 • φ2  • φ3 • φ4 ≺ Δ • φ.
 Proof.
 intros Hw1 Hw2 Hw3 Hw4 Hor.
-unfold env_order, ltof. repeat rewrite env_weight_add.
-apply env_le_weight in Hor.
+unfold env_order, ltof. repeat rewrite senv_weight_add.
+apply senv_le_weight in Hor.
 replace (weight φ) with (S (pred (weight φ))) by lia.
 apply Nat.lt_le_pred in Hw1, Hw2.
 simpl. repeat rewrite Nat.add_assoc.
@@ -246,8 +281,10 @@ Proof. etransitivity; [|apply env_order_0].	 assumption. Qed.
 
 Lemma env_order_eq_add Δ Δ' φ: (Δ ≼ Δ') -> (Δ • φ) ≼ (Δ' • φ).
 Proof. intros[Heq|Hlt]. left. now apply env_order_add_compat. right. ms. Qed.
+*)
+End Definitions.
 
-
+(*
 Global Hint Resolve env_order_0 : order.
 Global Hint Resolve env_order_1 : order.
 Global Hint Resolve env_order_2 : order.
@@ -270,8 +307,10 @@ Ltac get_diff_env g := match g with
 end.
 
 Global Hint Rewrite open_boxes_remove : order.
+*)
 
-Ltac prepare_order := 
+Ltac prepare_order := idtac.
+(*
 repeat (apply env_order_add_compat);
 unfold pointed_env_order; subst; simpl; repeat rewrite open_boxes_add; try match goal with
 | Δ := _ |- _ => subst Δ; try prepare_order
@@ -326,8 +365,72 @@ induction Δ using gmultiset_rec.
   + auto with *.
   + apply env_order_1. simpl. auto.
 Qed.
+*)
 
-Global Hint Resolve openboxes_env_order : order.
+Infix "≺·" := pointed_senv_order (at level 150).
+Global Hint Rewrite senv_weight_add : order.
+(* Global Hint Resolve openboxes_env_order : order. *)
+Global Hint Resolve senv_le_weight : order.
+Global Hint Unfold form_order : mset.
 
-Ltac order_tac := prepare_order; auto 10 with order.
+Lemma senv_order_remove_weak p d Δ φ:
+  (@senv_weight p (remove d φ Δ)) <= @senv_weight p Δ.
+Proof.
+unfold senv_weight.
+induction Δ as [| a Δ]; simpl.
+- constructor.
+- case d; intro; subst; simpl; lia.
+Qed.
 
+Lemma senv_order_remove p d Δ φ: φ ∈ Δ ->
+  pow_weight φ + (@senv_weight p (remove d φ Δ)) <= @senv_weight p Δ.
+Proof.
+intro Hin.
+induction Δ as [| a Δ]; simpl.
+- contradict Hin. auto with *.
+- rewrite senv_weight_add. case d; intro; subst; simpl.
+  + pose (senv_order_remove_weak d Δ a). lia.
+  + rewrite senv_weight_add.
+      apply elem_of_cons in Hin. destruct Hin as [Hf | Hin]; [tauto|].
+      specialize (IHΔ Hin). lia.
+Qed.
+
+
+(* TODO: technical. move *)
+
+Lemma lt_le_add_trans_r a b c x :(a <= b -> c < x + a -> c < x + b).
+Proof. lia. Qed.
+
+
+Ltac order_tac :=
+unfold pointed_senv_order;
+repeat (apply env_order_add_compat); simpl;
+unfold senv_order, ltof; repeat rewrite senv_weight_add;
+try match goal with | Δ := _ |- _ => subst Δ end;
+repeat match goal with
+  | Heq : existT ?a _ = existT ?a _ |- _ => apply Eqdep.EqdepTheory.inj_pair2 in Heq; subst
+  | Heq : existT ?n ?θ = _  |- _ =>
+   try subst n; try subst θ; inversion Heq;
+   rewrite <- sigT_eta in *; subst; simpl in * end;
+repeat rewrite Nat.add_assoc;
+   try match goal with Hin : ?ψ ∈ ?Γ |- context C [remove ?d ?ψ ?Γ] =>
+   eapply Nat.lt_le_trans; [| exact (senv_order_remove (nform_eq_dec _) Hin)] ||
+   eapply (lt_le_add_trans_r _ (senv_order_remove (nform_eq_dec _) Hin))
+end;
+repeat rewrite Nat.add_assoc;
+try refine (Nat.add_lt_le_mono _ _ _ _ _ (senv_weight_open_boxes _));
+unfold pow_weight, form_of_sig; simpl weight;
+repeat apply Nat.add_lt_mono_r;
+simpl Nat.pow;
+repeat rewrite ?Nat.pow_succ_r', ?Nat.pow_add_r;
+repeat match goal with
+|  |- context C [Nat.pow 5 (weight ?δ)] =>
+    lazymatch goal with 
+    | H :  5 <=  5 ^ (weight δ) |- _ => fail 
+    | _ => pose (pow_weight_gt δ) end end;
+simpl; unfold pow_weight in *; 
+try remember (senv_weight _) as W; try nia;
+try match goal with |- context C [?a * ?b * ?c] =>
+   (destruct (Nat.add_le_mul a b); [lia | lia | | lia]) end;
+ try eapply (lt_le_add_trans_r _ (senv_weight_open_boxes _));
+nia.
